moving SymEval2 to SymEval

MirrorCharge!/src/MirrorCharge/Imp/SymEval.v
@@ -1,3 +1,4 @@
+Require Import Coq.Strings.String.
 Require Import Coq.PArith.BinPos.
 Require Import ExtLib.Core.RelDec.
 Require Import ExtLib.Data.String.
@@ -13,208 +14,310 @@ Require Import MirrorCore.Subst.FMapSubst.
 Require Import MirrorCore.Lambda.ExprLift.
 Require Import MirrorCore.Lambda.ExprSubst.
 Require Import MirrorCore.Lambda.ExprUnify_simul.
-Require Import MirrorCharge.Imp.Imp.
+Require Import MirrorCore.Lambda.RedAll.
+Require Import MirrorCore.Lambda.AppN.
 Require Import MirrorCharge.ILogicFunc.
+Require Import MirrorCharge.OrderedCanceller.
+Require Import MirrorCharge.BILNormalize.
+Require Import MirrorCharge.SynSepLog.
+Require Import MirrorCharge.SepLogFold.
+Require MirrorCharge.Imp.Reify.
+Require Import MirrorCharge.Imp.Imp.
+Require Import MirrorCharge.Imp.Syntax.
+Require Import MirrorCharge.Imp.STacSimplify.
+(*Require Import MirrorCharge.Imp.STacCancel. *)
+Require Import MirrorCharge.Imp.STacCancelEx.
 
 Set Implicit Arguments.
 Set Strict Implicit.
 
-Section tactic.
+Local Existing Instance SS.
+Local Existing Instance SU.
+Local Existing Instance RSym_ilfunc.
+Local Existing Instance RS.
+Local Existing Instance Expr_expr.
 
-  Let subst : Type :=
-    FMapSubst.SUBST.raw (expr typ func).
-  Let SS : SubstI.Subst subst (expr typ func) :=
-    @FMapSubst.SUBST.Subst_subst _.
-  Let SU : SubstI.SubstUpdate subst (expr typ func) :=
-    FMapSubst.SUBST.SubstUpdate_subst (@instantiate typ func).
+Let EAPPLY lem tac :=
+  @EAPPLY typ (expr typ func) subst _ _ ExprLift.vars_to_uvars
+                (fun tus tvs n e1 e2 t s =>
+                   @exprUnify subst typ func _ _ RS SS SU 3 nil
+                              tus tvs n s e1 e2 t)
+                (@ExprSubst.instantiate typ func) SS SU
+                lem (apply_to_all tac).
 
-  Local Existing Instance SS.
-  Local Existing Instance SU.
-
-  Definition test_lemma :=
-    @lemmaD typ RType_typ (expr typ func) Expr_expr (expr typ func)
-            (fun tus tvs e => exprD' tus tvs e tyProp)
-            tyProp
-            (fun x => x) nil nil.
-
-
-  Definition fTriple : expr typ func := Inj (inl (inl 1%positive)).
-  Definition fSeq : expr typ func := Inj (inl (inl 2%positive)).
-  Definition fAssign : expr typ func := Inj (inl (inl 3%positive)).
-  Definition fRead : expr typ func := Inj (inl (inl 4%positive)).
-  Definition fVar (v : var) : expr typ func := Inj (inl (inr (pVar v))).
-  Definition fConst (c : nat) : expr typ func := Inj (inl (inr (pNat c))).
-  Definition fStar : expr typ func := Inj (inl (inl 5%positive)).
-  Definition fPtsTo : expr typ func := Inj (inl (inl 6%positive)).
-  Definition flocals_get : expr typ func := Inj (inl (inr pLocals_get)).
-  Definition flocals_upd : expr typ func := Inj (inl (inr pLocals_upd)).
-  Definition feval_iexpr : expr typ func := Inj (inl (inr pEval_expri)).
-  Definition fEq (t : typ) : expr typ func := Inj (inl (inr (pEq t))).
-
-  Definition mkTriple (P c Q : expr typ func) : expr typ func :=
-    App (App (App fTriple P) c) Q.
-  Definition mkSeq (a b : expr typ func) : expr typ func :=
-    App (App fSeq a) b.
-  Definition mkAssign (a b : expr typ func) : expr typ func :=
-    App (App fAssign a) b.
-  Definition mkRead (a b : expr typ func) : expr typ func :=
-    App (App fRead a) b.
-
-  (** NOTE: Manual lemma reification for the time being **)
-  Definition seq_lemma : lemma typ (expr typ func) (expr typ func) :=
-  {| vars := tyLProp :: tyLProp :: tyLProp :: tyCmd :: tyCmd :: nil
-   ; premises := mkTriple (Var 0) (Var 3) (Var 1) ::
-                 mkTriple (Var 1) (Var 4) (Var 2) :: nil
-   ; concl := mkTriple (Var 0) (mkSeq (Var 3) (Var 4)) (Var 2)
-   |}.
-
-  Definition seq_assoc_lemma : lemma typ (expr typ func) (expr typ func) :=
-  {| vars := tyLProp :: tyLProp :: tyCmd :: tyCmd :: tyCmd :: nil
-   ; premises :=
-       mkTriple (Var 0) (mkSeq (Var 2) (mkSeq (Var 3) (Var 4))) (Var 1) :: nil
-   ; concl :=
-       mkTriple (Var 0) (mkSeq (mkSeq (Var 2) (Var 3)) (Var 4)) (Var 1)
-   |}.
-
-  Let APPLY :=
-    @APPLY typ (expr typ func) subst _ Typ0_Prop
-           vars_to_uvars
-           (fun tus tvs n e1 e2 t s =>
-              @exprUnify subst typ func _ _ RS SS SU 3 nil
-                         tus tvs n s e1 e2 t)
-           (@instantiate typ func) SS SU.
-
-  Definition lex (l t : typ) (e : expr typ func) : expr typ func :=
-    App (Inj (inr (ilf_exists t l))) (Abs t e).
-
-  Definition lstar (l : typ) (e e' : expr typ func) : expr typ func :=
-    App (App fStar e) e'.
-  Definition land (l : typ) (e e' : expr typ func) : expr typ func :=
-    App (App (Inj (inr (ilf_and l))) e) e'.
-  Definition ltrue (l : typ) : expr typ func :=
-    Inj (inr (ilf_true l)).
-  Definition lentails (l : typ) (e e' : expr typ func) : expr typ func :=
-    App (App (Inj (inr (ilf_entails l))) e) e'.
-  Definition lor (l : typ) (e e' : expr typ func) : expr typ func :=
-    App (App (Inj (inr (ilf_or l))) e) e'.
-  Definition lembed (t f : typ) (e : expr typ func) : expr typ func :=
-    App (Inj (inr (ilf_embed f t))) e.
-  Definition lPtsTo (a b : expr typ func) : expr typ func :=
-    App (App fPtsTo a) b.
-
-  (** Assignment **)
-  Definition assign_lemma : lemma typ (expr typ func) (expr typ func) :=
-  {| vars := tyLProp :: tyVariable :: tyExpr :: nil
-   ; premises := nil
-   ; concl :=
-       mkTriple (Var 0)
-                (mkAssign (Var 1) (Var 2))
-                (Abs tyLocals
-                     (lex tyHProp tyNat
-                          (land tyHProp
-                                (lembed tyHProp tyProp
-                                        (App (App (fEq tyNat)
-                                                  (App (App flocals_get (Var 3)) (Var 1)))
-                                             (App (App feval_iexpr (Var 4)) (Var 1))))
-                                (App (Var 2) (App (App (App flocals_upd (Var 3)) (Var 0)) (Var 1))))))
-   |}.
-
-  Definition read_lemma : lemma typ (expr typ func) (expr typ func) :=
-  {| vars := tyLProp :: tyVariable :: tyExpr ::
-             tyArr tyLocals tyNat :: nil
-   ; premises :=
-       lentails tyLProp
-                (Var 0)
-                (Abs tyLocals
-                     (lstar tyHProp
-                            (App (App fPtsTo (App (App feval_iexpr (Var 3)) (Var 0))) (App (Var 4) (Var 0)))
-                            (ltrue tyHProp)))
-        :: nil
-   ; concl :=
-       mkTriple (Var 0)
-                (mkRead (Var 1) (Var 2))
-                (Abs tyLocals
-                     (lex tyHProp tyNat
-                          (land tyHProp
-                                (lembed tyHProp tyProp
-                                        (App (App (fEq tyNat)
-                                                  (App (App flocals_get (Var 3)) (Var 1)))
-                                             (App (Var 5) (App (App (App flocals_upd (Var 3)) (Var 0)) (Var 1)))))
-                                (App (Var 2) (App (App (App flocals_upd (Var 3)) (Var 0)) (Var 1))))))
-   |}.
-
-  Definition all_cases : stac typ (expr typ func) subst :=
-    REC 3 (fun rec =>
-             let rec := rec in
-             REPEAT 5
-                    (FIRST (   APPLY seq_assoc_lemma (apply_to_all rec)
-                            :: APPLY seq_lemma (apply_to_all rec)
-                            :: APPLY assign_lemma (apply_to_all rec)
-                            :: APPLY read_lemma (apply_to_all rec)
-                            :: nil)))
-        (@FAIL _ _ _).
-
-  Definition test :=
-    let vars := tyLProp :: tyCmd :: tyCmd :: tyCmd :: tyLProp :: nil in
-    let goal :=
-        mkTriple (Var 0)
-                 (mkSeq (mkSeq (Var 1) (Var 2)) (Var 3))
-                 (Var 4)
-    in
-    @all_cases nil vars (SubstI.empty (expr :=expr typ func)) nil goal.
-
-  Time Eval vm_compute in test.
-
-  Definition test' :=
-    let uvars := tyLProp :: nil in
-    let vars := tyLProp :: tyVariable :: tyCmd :: tyCmd :: tyLProp :: tyExpr :: nil in
-    let goal :=
-        mkTriple (Var 0)
-                 (mkSeq (mkAssign (Var 1) (Var 5)) (Var 2))
-                 (UVar 0)
-    in
-    @all_cases uvars vars (SubstI.empty (expr :=expr typ func)) nil goal.
-
-  Time Eval vm_compute in test'.
-
-  Local Notation "a @ b" := (@App typ _ a b) (at level 30).
-  Local Notation "\ t -> e" := (@Abs typ _ t e) (at level 40).
-
-  Definition test_read :=
-    let uvars := tyLProp :: nil in
-    let vars := tyVariable :: tyExpr :: nil in
-    let goal :=
-        mkTriple (Abs tyLocals (lPtsTo (App (App flocals_get (Var 1)) (Var 0)) (fConst 1)))
-                 (mkRead (Var 0) (Var 1))
-                 (UVar 0)
-    in
-    let tac :=
-        APPLY read_lemma (apply_to_all (@IDTAC _ _ _))
-    in
-    @tac uvars vars (SubstI.empty (expr :=expr typ func)) nil goal.
 (*
-  Time Eval cbv beta iota zeta delta - [ IDTAC ] in test_read.
+Definition texp (t : typ) : Type :=
+  expr typ func.
 *)
 
-  (** The next task is to automate the entailment
-   ** I'm going to have a goal that looks like this:
-   **   P |- Q
-   ** There are two approaches:
-   ** 1) Expose lambdas and go under the state.
-   **    This has the benefit that [star] looks like [star], there isn't
-   **    a bunch of lifting going on.
-   ** 2) Reason about the lifted logics explicitly.
-   **    This has the drawback that everything is lifted, so, e.g. instead
-   **    of seeing
-   **        (star P Q)
-   **    you will see
-   **        (ap (ap (pure star) P) Q)
-   ** If we do the former, then we need a way to put things back into a good
-   ** representation.
-   ** More of a problem is the fact that our unification variables will
-   ** need to mention the heap explicitly, i.e. we'll be working in two
-   ** unification contexts which substitutions can not handle at the moment.
-   ** ^--- This suggests that I *must* do the later.
-   **)
+Fixpoint get_alls (e : expr typ func) : list typ * expr typ func :=
+  match e with
+    | ExprCore.App (@ExprCore.Inj (inr (ILogicFunc.ilf_forall t tyProp)))
+                   (ExprCore.Abs _ e) =>
+      let (alls,e) := get_alls e in
+      (t :: alls, e)
+    | _ => (nil, e)
+  end.
 
-End tactic.
+Fixpoint get_impls (e : expr typ func) : list (expr typ func) * expr typ func :=
+  match e with
+    | ExprCore.App (ExprCore.App (Inj (inr (ILogicFunc.ilf_impl tyProp))) P) Q =>
+      let (impls,e) := get_impls Q in
+      (P :: impls,e)
+    | _ => (nil, e)
+  end.
+
+Definition convert_to_lemma (e : expr typ func)
+: lemma typ (expr typ func) (expr typ func) :=
+  let (alls, e) := get_alls e in
+  let (impls, e) := get_impls e in
+  {| vars := rev alls
+   ; premises := impls
+   ; concl := e |}.
+
+Ltac reify_lemma e :=
+  match type of e with
+    | ?T =>
+      (let k e :=
+           let e := constr:(convert_to_lemma e) in
+           let e := eval unfold convert_to_lemma in e in
+           let e := eval simpl in e in
+           refine e
+       in
+       reify_expr Reify.reify_imp k [ True ] [ T ])
+  end.
+
+(*
+Definition to_skip : lemma typ (expr typ func) (expr typ func) :=
+{| vars     := tyLProp :: tyCmd :: tyLProp :: tyLProp :: tySProp :: nil
+ ; premises := (Var 4 |- {{ Var 0 }} (Var 1) {{ Var 3 }}) ::
+               (Var 4 |- embed ((Var 2 : texp tyLProp) |- (Var 3))) :: nil
+ ; concl    := (Var 4 |- {{ Var 0 }} (Var 1) {{ Var 2 }}) : expr _ _
+ |}.
+
+Eval hnf in test_lemma to_skip.
+*)
+
+(** Skip **)
+Definition Skip_lemma : lemma typ (expr typ func) (expr typ func).
+reify_lemma Skip_rule.
+Defined.
+Print Skip_lemma.
+
+Theorem Skip_rule2
+: forall (G : SProp) P,
+    ILogic.lentails G (triple P Skip P).
+Proof.
+  intros. eapply Skip_rule.
+  (** TODO: How do I solve this? **)
+Admitted.
+
+Definition Skip_lemma2 : lemma typ (expr typ func) (expr typ func).
+reify_lemma Skip_rule2.
+Defined.
+Print Skip_lemma2.
+
+(** Sequence **)
+Definition Seq_lemma : lemma typ (expr typ func) (expr typ func).
+reify_lemma Seq_rule.
+Defined.
+Print Seq_lemma.
+
+Definition SeqA_lemma : lemma typ (expr typ func) (expr typ func).
+reify_lemma SeqA_rule.
+Defined.
+
+(** Assignment **)
+Definition Assign_lemma : lemma typ (expr typ func) (expr typ func).
+reify_lemma Assign_rule.
+Defined.
+Print Assign_lemma.
+(*
+{| vars := tyLProp :: tyVariable :: tyExpr :: nil
+ ; premises := nil
+ ; concl :=
+     mkTriple (Var 0)
+              (mkAssign (Var 1) (Var 2))
+              (lex tyLProp tyNat
+                   (land tyLProp
+                         (lap tyProp tyHProp
+                              (lpure (tyArr tyProp tyHProp) ((Inj (inr (ilf_embed tyProp tyHProp)))))
+                              (lap tyNat tyProp (lap tyNat (tyArr tyNat tyProp) (lpure (tyArr tyNat (tyArr tyNat tyProp))
+                                                                                       (fEq tyNat))
+                                                     (App flocals_get (Var 2)))
+                                   (lupdate tyNat (App (App flocals_upd (Var 2)) (Var 0)) (App feval_iexpr (Var 3)))))
+                         (lupdate tyHProp (App (App flocals_upd (Var 2)) (Var 0)) (Var 1))))
+ |}.
+*)
+
+(** Read **)
+Definition Read_lemma : lemma typ (expr typ func) (expr typ func).
+reify_lemma Read_rule.
+Defined.
+Print Read_lemma.
+(*
+{| vars := tyLProp :: tyVariable :: tyExpr ::
+                   tyArr tyLocals tyNat :: nil
+ ; premises :=
+     lentails tyLProp
+              (Var 0)
+              (lstar tyLProp
+                     (lap tyNat tyHProp (lap tyNat (tyArr tyNat tyHProp) (lpure (tyArr tyNat (tyArr tyNat tyHProp)) fPtsTo) (feval_iexpr @ Var 2)) (Var 3))
+                     (ltrue tyLProp))
+              :: nil
+ ; concl :=
+     mkTriple (Var 0)
+              (mkRead (Var 1) (Var 2))
+              (lex tyLProp tyNat
+                   (land tyLProp
+                         (lap tyProp tyHProp
+                              (lpure (tyArr tyProp tyHProp) ((Inj (inr (ilf_embed tyProp tyHProp)))))
+                              (lap tyNat tyProp (lap tyNat (tyArr tyNat tyProp) (lpure (tyArr tyNat (tyArr tyNat tyProp))
+                                                                                       (fEq tyNat))
+                                                     (App flocals_get (Var 2)))
+                                   (lupdate tyNat (App (App flocals_upd (Var 2)) (Var 0)) (Var 4))))
+                         (lupdate tyHProp (App (App flocals_upd (Var 2)) (Var 0)) (Var 1))))
+ |}.
+*)
+
+(** Write **)
+Definition Write_lemma : lemma typ (expr typ func) (expr typ func).
+reify_lemma Write_rule.
+Defined.
+Print Write_lemma.
+(*
+{| vars := tyLProp :: tyLProp :: tyExpr :: tyExpr :: nil
+ ; premises :=
+     lentails tyLProp
+              (Var 0)
+              (lex tyLProp tyNat
+                   (lstar tyLProp
+                          (lap tyNat tyHProp (lap tyNat (tyArr tyNat tyHProp)
+                                                  (lpure (tyArr tyNat (tyArr tyNat tyHProp)) fPtsTo)
+                                                  (feval_iexpr @ Var 3))
+                               (lpure tyNat (Var 0)))
+                          (Var 2)))
+     :: nil
+ ; concl :=
+     mkTriple (Var 0)
+              (mkWrite (Var 2) (Var 3))
+              (lstar tyLProp
+                     (lap tyNat tyHProp (lap tyNat (tyArr tyNat tyHProp) (lpure (tyArr tyNat (tyArr tyNat tyHProp)) fPtsTo) (feval_iexpr @ Var 2)) (feval_iexpr @ Var 3))
+                     (Var 1))
+ |}.
+*)
+
+(** Call **)
+Definition Call_lemma : lemma typ (expr typ func) (expr typ func).
+Abort.
+
+Definition solve_find_spec : stac typ (expr typ func) subst := FAIL.
+
+Definition solve_entailment :=
+  THEN (SIMPLIFY (fun _ _ _ => beta_all simplify nil nil))
+       stac_cancel.
+
+Definition all_cases : stac typ (expr typ func) subst :=
+  REC 2 (fun rec =>
+            let rec := rec in
+            REPEAT 5
+                   (FIRST (   EAPPLY SeqA_lemma rec
+                           :: EAPPLY Seq_lemma rec
+                           :: EAPPLY Assign_lemma rec
+                           :: EAPPLY Read_lemma solve_entailment
+                           :: EAPPLY Write_lemma solve_entailment
+                           :: EAPPLY Skip_lemma solve_entailment
+(*                           :: EAPPLY to_skip rec *)
+                           :: nil)))
+      (@FAIL _ _ _).
+
+Definition test :=
+  let vars := tyLProp :: tyCmd :: tyCmd :: tyCmd :: tyLProp :: tySProp :: nil in
+  let goal :=
+      Syntax.lentails tySProp
+                      (Var 5) (mkTriple (Var 0)
+                                        (mkSeq (mkSeq (Var 1) (Var 2)) (Var 3))
+                                        (Var 4))
+  in
+  @all_cases nil vars (SubstI.empty (expr :=expr typ func)) nil goal.
+
+Time Eval vm_compute in test.
+
+Definition test' :=
+  let uvars := tyLProp :: nil in
+  let vars := tyLProp :: tyVariable :: tyCmd :: tyCmd :: tyLProp :: tyExpr :: nil in
+  let goal :=
+      mkTriple (Var 0)
+               (mkSeq (mkAssign (Var 1) (Var 5)) (Var 2))
+               (UVar 0)
+  in
+  @all_cases uvars vars (SubstI.empty (expr :=expr typ func)) nil goal.
+
+Time Eval vm_compute in test'.
+
+Definition test_read_goal : expr typ func.
+
+Local Notation "a @ b" := (@App typ _ a b) (at level 30).
+Local Notation "'Ap' '[' x , y ']'" := (Inj (inl (inr (pAp x y)))) (at level 0).
+Local Notation "'Pure' '[' x ']'" := (Inj (inl (inr (pPure x)))) (at level 0).
+
+Definition test_read :=
+  let uvars := tyLProp :: nil in
+  let vars := nil in
+  let goal :=
+      mkTriple (lap tyNat tyHProp (lap tyNat (tyArr tyNat tyHProp) (lpure (tyArr tyNat (tyArr tyNat tyHProp)) fPtsTo)
+                                       (flocals_get @ fVar "p"))%string
+                    (lpure tyNat (fConst 1)))
+               (mkRead (fVar "x") (Inj (inl (inr eVar)) @ (fVar "p")))%string
+               (UVar 0)
+  in
+  let tac := all_cases in
+  @tac uvars vars (SubstI.empty (expr :=expr typ func)) nil goal.
+
+Time Eval vm_compute  in test_read.
+
+Definition lifted_ptsto (a b : expr typ func) : expr typ func :=
+  lap tyNat tyHProp (lap tyNat (tyArr tyNat tyHProp)
+                         (lpure (tyArr tyNat (tyArr tyNat tyHProp)) fPtsTo)
+                         a) b.
+
+Definition test_read2 :=
+  let uvars := tyLProp :: nil in
+  let vars := tyNat :: tyNat :: nil in
+  let goal :=
+      (mkTriple
+         (lstar tyLProp
+                (lifted_ptsto (flocals_get @ fVar "p1") (lpure tyNat (Var 0)))
+                (lifted_ptsto (flocals_get @ fVar "p2") (lpure tyNat (Var 1))))
+         (mkSeq (mkRead (fVar "t1") (Inj (inl (inr eVar)) @ (fVar "p1")))
+                (mkRead (fVar "t2") (Inj (inl (inr eVar)) @ (fVar "p2"))))
+         (UVar 0))%string
+  in
+  let tac := all_cases in
+  @tac uvars vars (SubstI.empty (expr :=expr typ func)) nil goal.
+
+Eval cbv beta iota zeta delta in test_read2.
+
+Definition test_swap :=
+  let uvars := nil in
+  let vars := tyNat :: tyNat :: nil in
+  let goal :=
+      (mkTriple
+         (lstar tyLProp
+                (lifted_ptsto (flocals_get @ fVar "p1") (lpure tyNat (Var 0)))
+                (lifted_ptsto (flocals_get @ fVar "p2") (lpure tyNat (Var 1))))
+         (mkSeq (mkRead (fVar "t1") (Inj (inl (inr eVar)) @ (fVar "p1")))
+         (mkSeq (mkRead (fVar "t2") (Inj (inl (inr eVar)) @ (fVar "p2")))
+         (mkSeq (mkWrite (Inj (inl (inr eVar)) @ fVar "p2") (Inj (inl (inr eVar)) @ (fVar "t1")))
+                (mkWrite (Inj (inl (inr eVar)) @ fVar "p1") (Inj (inl (inr eVar)) @ (fVar "t2"))))))
+         (lstar tyLProp
+                (lifted_ptsto (flocals_get @ fVar "p1") (lpure tyNat (Var 1)))
+                (lifted_ptsto (flocals_get @ fVar "p2") (lpure tyNat (Var 0)))))%string
+  in
+  let tac := all_cases in
+  @tac uvars vars (SubstI.empty (expr :=expr typ func)) nil goal.
+
+Eval vm_compute in test_swap.
+(** This is not the strongest post condition because we forgot the pure facts.
+ ** This is likely a problem with the cancellation algorithm.
+ **)
